<?xml version="1.0"?>

<rdf:RDF
  xml:lang="en"
  xmlns:rdf="http://www.w3.org/1999/02/22-rdf-syntax-ns#"
  xmlns:rdfs="http://www.w3.org/2000/01/rdf-schema#"
  xmlns:skos="http://www.w3.org/2004/02/skos/core#"
  xmlns:boltz="http://solid.boltz.cs.cmu.edu:3030/"
  xmlns:kgo="http://solid.boltz.cs.cmu.edu:3030/ontology#">

  <rdfs:Class rdf:about='http://solid.boltz.cs.cmu.edu:3030/Q530397'>
    <rdfs:comment>This is the base class that comes up on KBPedia when you search for Alligator</rdfs:comment>
    <rdfs:subClassOf rdf:resource="http://solid.boltz.cs.cmu.edu:3030/ontology#Taxon"/>
    <skos:definition>The collection of all alligators; a subset of Crocodilian. Alligator includes the American Alligators and Chinese Alligators. Cf. Crocodile.</skos:definition>
    <skos:prefLabel>Alligator</skos:prefLabel>
    <kgo:taxonRank rdf:resource="http://solid.boltz.cs.cmu.edu:3030/ontology#Genus"/>
    <kgo:superTaxonOf rdf:resource='http://solid.boltz.cs.cmu.edu:3030/Q193327'/>
    <kgo:superTaxonOf rdf:resource='http://solid.boltz.cs.cmu.edu:3030/Q194422'/>
  </rdfs:Class>

  <rdfs:Class rdf:about='http://solid.boltz.cs.cmu.edu:3030/Q193327'>
    <rdfs:comment>Note that subClassOf Animal is from the Test dataset</rdfs:comment>
    <rdfs:subClassOf rdf:resource="http://www.w3.org/2000/03/example/classes#Animal"/>
    <rdfs:subClassOf rdf:resource="http://solid.boltz.cs.cmu.edu:3030/ontology#Taxon"/>
    <skos:definition>The American alligator (Alligator mississippiensis), sometimes referred to colloquially as a gator or common alligator, is a large crocodilian reptile endemic to the southeastern United States. It is one of two living species in the
      genus Alligator within the family Alligatoridae; it is larger than the other extant alligator species, the Chinese alligator. Adult male American alligators measure 3.4 to 4.6 m (11 to 15 ft) in length, and can weigh up to 453 kg (1,000 lb). Females
      are smaller, measuring around 3 m (9.8 ft). The American alligator inhabits freshwater wetlands, such as marshes and cypress swamps from Texas to North Carolina. It is distinguished from the sympatric American crocodile by its broader snout, with
      overlapping jaws and darker coloration, and is less tolerant of saltw.</skos:definition>
    <skos:prefLabel>American Alligator</skos:prefLabel>
    <kgo:taxonRank rdf:resource="http://solid.boltz.cs.cmu.edu:3030/ontology#Species"/>
    <kgo:taxonName>Alligator mississippiensis</kgo:taxonName>
    <kgo:subTaxonOf rdf:resource="http://solid.boltz.cs.cmu.edu:3030/Q530397"/>
  </rdfs:Class>

  <rdfs:Class rdf:about='http://solid.boltz.cs.cmu.edu:3030/Q194422'>
    <rdfs:comment>Note that subClassOf Animal is from the Test dataset</rdfs:comment>
    <rdfs:subClassOf rdf:resource="http://www.w3.org/2000/03/example/classes#Animal"/>
    <rdfs:subClassOf rdf:resource="http://solid.boltz.cs.cmu.edu:3030/ontology#Taxon"/>
    <skos:definition>The Chinese alligator (Alligator sinensis) (simplified Chinese: 扬子鳄; traditional Chinese: 揚子鱷, yáng zǐ è), also known as the Yangtze alligator, is one of two known living species of Alligator, a genus in the family Alligatoridae.
      This critically endangered species is endemic to eastern China.</skos:definition>
    <skos:prefLabel>Chinese Alligator</skos:prefLabel>
    <kgo:taxonRank rdf:resource="http://solid.boltz.cs.cmu.edu:3030/ontology#Species"/>
    <kgo:taxonName>Alligator sinensis</kgo:taxonName>
    <kgo:subTaxonOf rdf:resource="http://solid.boltz.cs.cmu.edu:3030/Q530397"/>
  </rdfs:Class>

</rdf:RDF>
